test/chain_trans.lean
@@ -2,21 +2,24 @@
 import tactic.chain_trans
 import tactic.interactive
 
+/-- long chain of inequalities with a mix of `≤`, `<` and `=` -/
 example {x y z w u v : ℕ} {a b : ℤ} (h₀ : x ≤ y) (h₁ : y < z) (h : y < u) (h₂ : z < w) (h₃ : w = u) (h₄ : u < v) : x ≤ u :=
 begin
   chain_trans,
 end
 
+/-- error message when `≤` can be proved but not `<` -/
 example {w x y z : ℕ} {a b : ℤ} (h₀ : w ≤ x) (h₁ : x = y) (h₂ : y < z) : true :=
 begin
   have : w < w,
   { success_if_fail_with_msg
     { chain_trans }
-    "no appropriate chain of inequalities can be found between `w` and `w`",
+    "`w < w` cannot be proved from `w ≤ w`",
     admit },
   triv
 end
 
+/-- error message when no proof is found -/
 example {w x y z : ℕ} {a b : ℤ} (h₀ : w ≤ x) (h₁ : x = y) (h₂ : y < z) : true :=
 begin
   have : x < w,
@@ -27,12 +30,20 @@ begin
   triv
 end
 
+/-- simple example -/
 example {w x y z : ℕ} {a b : ℤ} (h₀ : w ≤ x) (h₁ : x = y) (h₂ : y < z) : w < z :=
 begin
   chain_trans,
 end
 
+/-- there exists a proof of `w ≤ z` and one of `w < z`. `chain_trans` should prefer `w < z` -/
 example {w x y z : ℕ} {a b : ℤ} (h₀ : w ≤ x) (h₁ : y = z) (h₃ : x ≤ y) (h₂ : x < y) (h₃ : x ≤ y) : w < z :=
+begin
+  chain_trans,
+end
+
+/-- normalize vertices using `whnf` to recognize definitionally equal terms -/
+example {w x y z : ℕ} {a b : ℤ} (h₀ : w ≤ x) (h₁ : y = id z) (h₃ : x ≤ y) (h₂ : id x < y) (h₃ : x ≤ y) : w < z :=
 begin
   chain_trans,
 end
